backend/Mach.v
@@ -269,7 +269,7 @@ Inductive state: Type :=
              (m: mem),                 (**r memory state *)
         state.
 
-Definition Mach_get_mem (s:state):=
+Definition get_mem (s:state):=
   match s with
   | State _ _ _ _ _ m => m
   | Callstate _ _ _ m => m
