cfrontend/Csharpminor.v
@@ -168,7 +168,7 @@ Inductive state: Type :=
         state.
 
 
-Definition Csharpminor_get_mem (s:state):=
+Definition get_mem (s:state):=
   match s with
   | State _ _ _ _ _ m => m
   | Callstate _ _ _ m => m
