backend/Allocproof.v
@@ -16,7 +16,7 @@
 Require Import FSets.
 Require Import Coqlib Ordered Maps Errors Integers Floats.
 Require Import AST Linking Lattice Kildall.
-Require Import Values Memory Globalenvs Events Smallstep.
+Require Import Values Memory Globalenvs Events Smallstep ExposedSmallstep2.
 Require Archi.
 Require Import Op Registers RTL Locations Conventions RTLtyping LTL.
 Require Import Allocation.
@@ -2305,5 +2305,37 @@ Proof.
   eapply subject_reduction; eauto. eexact wt_prog. eexact H.
   auto.
 Qed.
+
+Theorem transl_program_correct':
+  @fsim_properties  (RTL.semantics prog) (LTL.semantics tprog)
+                  (Smallstep.state (RTL.semantics prog)) (ltof _ (fun _ => 0)%nat)
+                  ( fun idx s1 s2 => idx = s1 /\ ( wt_state s1 /\ match_states s1 s2)).
+Proof.
+  eapply forward_simulation_plus'.
+- apply senv_preserved.
+- intros. exploit initial_states_simulation; eauto. intros [st2 [A B]].
+  exists st2; split; auto. split; auto.
+  apply wt_initial_state with (p := prog); auto. exact wt_prog.
+- intros. destruct H. eapply final_states_simulation; eauto.
+- intros. destruct H0.
+  exploit step_simulation; eauto. intros [s2' [A B]].
+  exists s2'; split. exact A. split.
+  eapply subject_reduction; eauto. eexact wt_prog. eexact H.
+  auto.
+Qed.
+
+Theorem transl_program_correct'':
+  @fsim_properties_ext
+    (RTL.semantics prog) (LTL.semantics tprog)
+    RTL.get_mem LTL.get_mem
+    (Smallstep.state (RTL.semantics prog)) (ltof _ (fun _ => 0)%nat)
+    ( fun idx s1 s2 => idx = s1 /\ ( wt_state s1 /\ match_states s1 s2)).
+Proof.
+  eapply sim_extSim.
+  - simpl; intros ? ? ? [? ?]; subst.
+    destruct H0 as [? H0]; inversion H0; auto.
+  - apply transl_program_correct'.
+Qed.
+
 
 End PRESERVATION.
