backend/CSEproof.v
@@ -14,7 +14,7 @@
 
 Require Import Coqlib Maps Errors Integers Floats Lattice Kildall.
 Require Import AST Linking.
-Require Import Values Memory Events Globalenvs Smallstep.
+Require Import Values Memory Events Globalenvs Smallstep ExposedSmallstep2.
 Require Import Op Registers RTL.
 Require Import ValueDomain ValueAOp ValueAnalysis.
 Require Import CSEdomain CombineOp CombineOpproof CSE.
@@ -1236,6 +1236,33 @@ Proof.
 - intros. destruct H. eapply transf_final_states; eauto.
 - intros. destruct H0. exploit transf_step_correct; eauto.
   intros [s2' [A B]]. exists s2'; split. auto. split. eapply sound_step; eauto. auto.
+Qed.
+
+Theorem transl_program_correct':
+  @fsim_properties  (RTL.semantics prog) (RTL.semantics tprog)
+                  (Smallstep.state (RTL.semantics prog)) (ltof _ (fun _ => 0)%nat)
+                  ( fun idx s1 s2 => idx = s1 /\ (sound_state prog s1 /\ match_states s1 s2)).
+Proof.
+  eapply forward_simulation_step'. 
+- apply senv_preserved.
+- intros. exploit transf_initial_states; eauto. intros [s2 [A B]].
+  exists s2. split. auto. split. apply sound_initial; auto. auto.
+- intros. destruct H. eapply transf_final_states; eauto.
+- intros. destruct H0. exploit transf_step_correct; eauto.
+  intros [s2' [A B]]. exists s2'; split. auto. split. eapply sound_step; eauto. auto.
+Qed.
+
+Theorem transl_program_correct'':
+  @fsim_properties_ext
+    (RTL.semantics prog) (RTL.semantics tprog)
+    RTL.get_mem RTL.get_mem
+                  (Smallstep.state (RTL.semantics prog)) (ltof _ (fun _ => 0)%nat)
+                  ( fun idx s1 s2 => idx = s1 /\ (sound_state prog s1 /\ match_states s1 s2)).
+Proof.
+  eapply sim_extSim.
+  - simpl; intros ? ? ? [? ?]; subst.
+    destruct H0 as [? H0]; inversion H0; auto.
+  - apply transl_program_correct'.
 Qed.
 
 End PRESERVATION.
