backend/Renumberproof.v
@@ -14,7 +14,7 @@
 
 Require Import Coqlib Maps Postorder.
 Require Import AST Linking.
-Require Import Values Memory Globalenvs Events Smallstep.
+Require Import Values Memory Globalenvs Events Smallstep ExposedSmallstep2.
 Require Import Op Registers RTL Renumber.
 
 Definition match_prog (p tp: RTL.program) :=
@@ -259,11 +259,29 @@ Proof.
   exact step_simulation.
 Qed.
 
+Theorem transl_program_correct':
+  fsim_properties  (RTL.semantics prog) (RTL.semantics tprog)
+                  _ (ltof _ ( fun _ => O))
+(fun idx s1 s2 => idx = s1 /\ match_states s1 s2).
+Proof.
+  eapply forward_simulation_step'.
+  apply senv_preserved.
+  eexact transf_initial_states.
+  eexact transf_final_states.
+  exact step_simulation.
+Qed.
+
+Theorem transl_program_correct'':
+  @fsim_properties_ext  (RTL.semantics prog) (RTL.semantics tprog)
+                        RTL.get_mem RTL.get_mem
+                        _ (ltof _ ( fun _ => O))
+(fun idx s1 s2 => idx = s1 /\ match_states s1 s2).
+Proof.
+  eapply EqEx_sim'; eapply sim_eqSim'.
+  - simpl; intros ? ? ? [? ?].
+    inversion H0; reflexivity.
+  - apply transl_program_correct'.
+Qed.
+
 End PRESERVATION.
-
-
-
-
-
-
 
