backend/Tailcallproof.v
@@ -13,7 +13,7 @@
 (** Recognition of tail calls: correctness proof *)
 
 Require Import Coqlib Maps Integers AST Linking.
-Require Import Values Memory Events Globalenvs Smallstep.
+Require Import Values Memory Events Globalenvs Smallstep ExposedSmallstep2.
 Require Import Op Registers RTL Conventions Tailcall.
 
 (** * Syntactic properties of the code transformation *)
@@ -601,6 +601,31 @@ Proof.
   eexact transf_initial_states.
   eexact transf_final_states.
   exact transf_step_correct.
+Qed.
+
+
+Theorem transl_program_correct':
+  fsim_properties  (RTL.semantics prog) (RTL.semantics tprog)
+                  _ (ltof _ measure)
+(fun idx s1 s2 => idx = s1 /\ match_states s1 s2).
+Proof.
+  eapply forward_simulation_opt' with (measure := measure); eauto.
+  apply senv_preserved. 
+  eexact transf_initial_states.
+  eexact transf_final_states.
+  exact transf_step_correct.
+Qed.
+
+Theorem transl_program_correct'':
+  @fsim_properties_ext  (RTL.semantics prog) (RTL.semantics tprog)
+                       RTL.get_mem RTL.get_mem
+                  _ (ltof _ measure)
+(fun idx s1 s2 => idx = s1 /\ match_states s1 s2).
+Proof.
+  eapply sim_extSim.
+  - simpl; intros ? ? ? [? ?]; subst.
+    inversion H0; simpl; auto.
+  - apply transl_program_correct'.
 Qed.
 
 End PRESERVATION.
