backend/Tunnelingproof.v
@@ -14,7 +14,7 @@
 
 Require Import Coqlib Maps UnionFind.
 Require Import AST Linking.
-Require Import Values Memory Events Globalenvs Smallstep.
+Require Import Values Memory Events Globalenvs Smallstep ExposedSmallstep2.
 Require Import Op Locations LTL.
 Require Import Tunneling.
 
@@ -406,6 +406,32 @@ Proof.
   eexact transf_initial_states.
   eexact transf_final_states.
   eexact tunnel_step_correct.
+Qed.
+
+
+Theorem transl_program_correct':
+  @fsim_properties  (LTL.semantics prog) (LTL.semantics tprog)
+                  _ (ltof _ measure)
+                  ( fun idx s1 s2 => idx = s1 /\ match_states s1 s2).
+Proof.
+  eapply forward_simulation_opt'.
+  apply senv_preserved.
+  eexact transf_initial_states.
+  eexact transf_final_states.
+  eexact tunnel_step_correct.
+Qed.
+
+Theorem transl_program_correct'':
+  @fsim_properties_ext
+    (LTL.semantics prog) (LTL.semantics tprog)
+    LTL.get_mem LTL.get_mem
+                  _ (ltof _ measure)
+                  ( fun idx s1 s2 => idx = s1 /\ match_states s1 s2).
+Proof.
+  eapply EqEx_sim'; eapply sim_eqSim'.
+  - simpl; intros ? ? ? [? ?]; subst.
+    destruct H0; auto.
+  - apply transl_program_correct'.
 Qed.
 
 End PRESERVATION.
